practice/NOC_setup2.v
@@ -1,0 +1,73 @@
+Require Import Koika.Frontend.
+Require Import Koika.Std.
+Require Import Router.
+Require Import Types.
+From Coq Require Import Arith Lia Program.
+From Equations Require Import Equations.
+Require Import Coq.Vectors.Fin.
+
+Module Type NOC_data.
+  Parameter nocsize: nat.
+  Axiom nocprop: 1<nocsize.
+End NOC_data.
+
+Module NOCSetup(ND:NOC_data)(MyTypes: Typesize).
+Import ND. 
+Module NOC_type := Types(MyTypes).
+Import NOC_type.
+Definition interfacesize := Nat.mul nocsize 2. 
+Definition regno := Nat.add nocsize (Nat.sub nocsize 1).
+
+Definition regno' (r:nat):= Nat.add r (Nat.sub r 1).
+Definition interfacesize' (nocsize:nat) := Nat.mul nocsize 2. 
+Inductive reg_t := reg_ (n: Fin.t regno).
+Inductive rule_name_t := rule_ (n: Fin.t regno).
+Inductive ext_fn_t := ex_ (n: Fin.t regno).
+
+
+Module MyRegs <: Registers.
+Definition reg_t:=reg_t.
+Definition ext_fn_t:= ext_fn_t.
+End MyRegs.
+
+Module Routerfns:= Router(MyRegs)(MyTypes).        
+Import Routerfns.
+
+Fixpoint fin_to_nat {n : nat} (f : Fin.t n) : nat :=
+  match f with
+  | Fin.F1 => 0
+  | Fin.FS f' => S (fin_to_nat f')
+end.
+
+Definition nat_to_fin {n : nat} (i : nat) (pf : i < n) : Fin.t n :=
+  Fin.of_nat_lt pf. 
+
+Equations? to_action (nocsize:nat) (H: 2<=nocsize) (rl : rule_name_t) :
+uaction reg_t ext_fn_t:=
+    
+   to_action 1 (le_S nocsize H1) _ with H1 := {} ; 
+   to_action (S nocsize') H (rule_ idx) :=
+       let n_idx := fin_to_nat idx in
+       (* let interfacesize := Nat.mul nocsize' 2 in 
+       let regno := Nat.add (S nocsize') (Nat.sub (S nocsize') 1) in *)
+       if Nat.eqb n_idx 0 then
+                     routestartfn 0 
+                           (reg_ (nat_to_fin 0 _)) 
+                           (reg_ (nat_to_fin nocsize' _)) 
+                           (ex_ (nat_to_fin 0 _)) 
+                           (ex_ (nat_to_fin 1 _))
+       else if Nat.eqb n_idx nocsize' then
+                     routeendfn nocsize'
+                           (reg_ (nat_to_fin (Nat.pred n_idx) _ ))
+                           (reg_ (nat_to_fin  (Nat.add (Nat.pred n_idx) nocsize') _))
+                           (ex_  (nat_to_fin (Nat.mul n_idx 2) _ )) 
+                           (ex_  (nat_to_fin (S (Nat.mul n_idx 2)) _))
+       else
+                      routecenterfn n_idx 
+                           (reg_ (nat_to_fin (Nat.pred n_idx) _ ))
+                           (reg_ (nat_to_fin  n_idx _))
+                           (reg_ (nat_to_fin  (Nat.add (Nat.pred n_idx) nocsize') _))
+                           (ex_ (nat_to_fin (Nat.mul n_idx 2) _ )) 
+                           (ex_ (nat_to_fin (S (Nat.mul n_idx 2)) _)).
+Proof.
+- unfold regno.
