practice/rough.v
@@ -1,0 +1,447 @@
+Require Import Koika.Frontend.
+Require Import Koika.Std.
+Require Import Router.
+Require Import Types.
+From Coq Require Import Arith Lia Program.
+From Equations Require Import Equations.
+Require Import Coq.Vectors.Fin.
+
+Module Type NOC_data.
+  Parameter nocsize: nat.
+  Axiom nocprop: 1<nocsize.
+End NOC_data.
+
+Module NOCSetup(ND:NOC_data)(MyTypes: Typesize).
+Import ND. 
+Module NOC_type := Types(MyTypes).
+Import NOC_type.
+Definition interfacesize := Nat.mul nocsize 2. 
+Definition regno := Nat.add nocsize (Nat.sub nocsize 1).
+
+Definition regno' := fun nsize => nsize + (nsize-1).
+
+
+Inductive reg_t : nat -> Type :=
+  | reg_ : forall num, Fin.t num -> reg_t num.
+
+  Inductive rule_name_t : nat -> Type :=
+  | rule_ : forall num, Fin.t num -> rule_name_t num.
+
+  Inductive ext_fn_t : nat -> Type :=
+  | ex_ : forall num, Fin.t num -> ext_fn_t num.
+
+(* Inductive reg_t: nat->Type := reg_ (n: Vect.index regno).
+Inductive rule_name_t := rule_ (n: Vect.index nocsize).
+
+Inductive ext_fn_t := ex_ (n: Vect.index interfacesize). *)
+
+Module MyRegs <: Registers.
+Definition reg_t:=reg_t (regno' nocsize).
+Definition ext_fn_t:= ext_fn_t interfacesize.
+End MyRegs.
+
+Module Routerfns:= Router(MyRegs)(MyTypes).        
+Import Routerfns.
+
+Locate "<".
+Print lt.
+Locate "<=".
+Print le.
+Locate "<>".
+Print not. 
+
+ (* Fixpoint nat_to_fin {n : nat} (m : nat) : option (Fin.t n) :=
+  match n return option (Fin.t n) with
+  | 0 => None (* No valid index if the bound is 0 *)
+  | S n' => match m with
+            | 0 => Some Fin.F1 (* The 0th index corresponds to Fin.F1 *)
+            | S m' => match nat_to_fin m' with
+                      | Some fin' => Some (Fin.FS fin') (* Successor index *)
+                      | None => None
+                      end
+            end
+  end. *)
+
+  Check Nat.nlt_0_r.
+  Check Fin.of_nat.
+  Check Fin.of_nat_lt.
+
+  Definition nat_to_fin {n : nat} (i : nat) (pf : i < n) : Fin.t n :=
+    Fin.of_nat_lt pf. 
+  
+  Check Nat.nlt_0_r.
+
+  Example example_fin_auto : 2 < 7.
+Proof.
+  info_auto 8. (* auto and info_auto dont work for some numbers*)
+Qed.
+
+Fixpoint fin_to_nat {n : nat} (f : Fin.t n) : nat :=
+  match f with
+  | Fin.F1 => 0
+  | Fin.FS f' => S (fin_to_nat f')
+  end.
+
+Compute Fin.of_nat_lt example_fin_auto.
+Compute @nat_to_fin 7 1 _.
+Check nat_to_fin.
+Compute Fin.of_nat_lt example_fin_auto.  
+Compute fin_to_nat (Fin.FS Fin.F1).
+(* Check rule_ nocsize Fin.F1. *)
+
+(* Equations get_rule {nocsize:nat} (H: 1<=nocsize) (idx:Fin.t nocsize) : rule_name_t nocsize :=
+  (* get_rule 0   -> dicharged by equations *)
+  @get_rule (S n) _ idx := rule_ (S n) idx.
+
+Definition idx_zero (n:nat) : Fin.t (S n) := Fin.F1.
+Definition idx_one (n:nat) : Fin.t (S (S n)) := Fin.FS (idx_zero n).
+
+Definition lower_bound : Fin.t 4 := Fin.FS (Fin.FS (Fin.FS Fin.F1)).
+Print lower_bound.
+Print vect_nil.
+Print Fin.t.
+Inductive vec (T:Type) : nat -> Type :=
+  | vec_nil : vec T 0
+  | vec_append : forall n, T -> vec T n -> vec T (S n).
+
+Inductive myfin : nat -> Type :=
+  | myf1 : forall n, myfin (S n)
+  | myfs : forall n, myfin n -> myfin (S n).
+
+Check Fin.F1.
+
+Definition t_2 : Fin.t 3 :=  (Fin.FS (Fin.FS Fin.F1)).
+Equations idx' {n:nat} (i:Fin.t n) (ub:nat) :Fin.t n :=
+let 
+  idx' i'  0    := i';
+  idx' i' (S n) := idx' (Fin.FS i') n. 
+
+Equations idx (i:nat) (upper_bound:nat) (H: i<upper_bound)(H2: upper_bound>0) : Fin.t (S upper_bound) :=
+  idx 0 ub _ _ := @Fin.F1 ub;
+  idx (S n)
+
+Equations idx (i:nat) (sz:nat) (H: i<sz)(H2: sz>0)  : Fin.t sz :=
+  idx 0 _ _ _ := Fin.F1;
+  idx (S n) sz _ _ := @Fin.FS (S n) (idx n sz _ _ ).
+
+Equations rule_1 (nocsize:nat) (H: 1<=nocsize) (idx:Fin.t n) :rule_name_t nocsize:=
+  (* rule_1 0   *)
+  rule_1 (S 0) (le_S n H1) _ with H1 := {};
+  rule_1 (S (S n)) := rule_ nocsize (Fin.FS (Fin.FS (Fin.F1 n)). *)
+Search Fin.t.
+Compute Nat.pred nocsize.
+Compute Nat.mul 2 3.
+
+
+
+Lemma regno_gt_0 : 0 < regno.
+Proof.
+  unfold regno.
+  apply Nat.add_pos_pos.
+  - apply Nat.lt_le_incl. exact nocprop.
+  - 
+    assert (aaa : 1 < nocsize). { exact nocprop. }
+    destruct nocsize.
+    + inversion aaa.
+    + simpl. 
+      rewrite Nat.sub_0_r.
+      apply Nat.succ_lt_mono.
+      exact aaa.
+Qed.
+
+Equations? to_action (nocsize:nat) (H: 2<=nocsize) (rl : rule_name_t nocsize) :
+ uaction (reg_t regno) (ext_fn_t interfacesize) :=
+     
+    to_action 1 (le_S nocsize H1) _ with H1 := {} ; 
+    to_action (S nocsize') H (rule_ nocsize' idx) :=
+        let n_idx := fin_to_nat idx in
+        (* let interfacesize := Nat.mul nocsize' 2 in 
+        let regno := Nat.add (S nocsize') (Nat.sub (S nocsize') 1) in *)
+        if Nat.eqb n_idx 0 then
+                      routestartfn 0 
+                            (reg_ (regno' nocsize) (nat_to_fin 0 _)) 
+                            (reg_ (regno' nocsize) (nat_to_fin nocsize' _)) 
+                            (ex_ interfacesize (nat_to_fin 0 _)) 
+                            (ex_ interfacesize (nat_to_fin 1 _))
+        else if Nat.eqb n_idx nocsize' then
+                      routeendfn nocsize'
+                            (reg_ regno (nat_to_fin (Nat.pred n_idx) _ ))
+                            (reg_ regno (nat_to_fin  (Nat.add (Nat.pred n_idx) nocsize') _))
+                            (ex_ interfacesize (nat_to_fin (Nat.mul n_idx 2) _ )) 
+                            (ex_ interfacesize (nat_to_fin (S (Nat.mul n_idx 2)) _))
+        else
+                       routecenterfn n_idx 
+                            (reg_ regno (nat_to_fin (Nat.pred n_idx) _ ))
+                            (reg_ regno (nat_to_fin  n_idx _))
+                            (reg_ regno (nat_to_fin  (Nat.add (Nat.pred n_idx) nocsize') _))
+                            (ex_ interfacesize (nat_to_fin (Nat.mul n_idx 2) _ )) 
+                            (ex_ interfacesize (nat_to_fin (S (Nat.mul n_idx 2)) _)).
+ - apply regno_gt_0.
+ - unfold regno.
+Qed.
+apply regno_gt_0.
+Next Obligation.
+
+Search nocsize.
+Check le_plus_trans.
+apply le_plus_l, nocprop.
+Search plus.
+apply nocprop.
+omega.
+Check le_S.
+Check le_n.  
+replace (nocsize + (nocsize - 1)) with (2 * nocsize - 1).
+apply Nat.lt_le_incl.
+
+Search nat. 
+Check Nat.lt.
+Check Nat.lt_le_incl.
+Check Nat.lt_alt.
+
+apply Nat.lt_le_incl.
+
+
+
+
+
+
+Definition R ( reg : reg_t regno ) :=
+  match reg with
+  |  _ => bits_t (struct_sz basic_flit)
+  end.
+  
+Definition r (reg : reg_t regno) : R reg :=
+  match reg with
+  |  _ => Bits.zero
+  end.
+
+Definition Sigma' (fn: ext_fn_t interfacesize) : ExternalSignature :=
+  match fn with
+  | _ => {$ bits_t sz ~> bits_t sz $}
+  end.
+
+End NOCSetup.
+  (* Check tc_rules. *)
+(* 
+  Definition rules :=
+  tc_rules R Sigma'  to_action. *)
+
+(* Equations to_action' (nocsize:nat) (H: 1<=nocsize) (rl : rule_name_t nocsize) : uaction (reg_t regno) (ext_fn_t interfacesize) := 
+  (* to_action 0 H _ := { }; *)
+   to_action 1 (le_S n H1) _ with H1 := {} ; 
+   let idx := nat_to_fin nocsize 
+
+  to_action' (S nocsize') H (rule_ nocsize Fin.F1) :=
+    routestartfn 0 
+                (reg_ regno (nat_to_fin 0 _)) 
+                (reg_ regno (nat_to_fin nocsize' _)) 
+                (ex_ interfacesize (nat_to_fin 0 _)) 
+                (ex_ interfacesize (nat_to_fin 1 _));
+
+  to_action' (S nocsize') H (rule_ (S nocsize) n)  with n == (nat_to_fin nocsize') :=
+    | := routerend ...
+    | nocsize H (rule_ nocsize idx) :=
+        let n_idx := fin_to_nat idx in
+        routecenterfn n_idx 
+                (reg_ regno (nat_to_fin (Nat.pred n_idx) _ ))
+                (reg_ regno (nat_to_fin  n_idx _))
+                (reg_ regno (nat_to_fin  (Nat.add (Nat.pred n_idx) nocsize) _))
+                (ex_ interfacesize (nat_to_fin (Nat.mul n_idx 2) _ )) 
+                (ex_ interfacesize (nat_to_fin (S (Nat.mul n_idx 2)) _)).
+(* to_action nocsize H (rule_ nocsize n) := routecenterfn n (reg_ n) (reg_ (Nat.add nocsize n) ex_ 2n ex_ 2n+1) *)
+
+Equations to_action (nocsize:nat) (H: 2<=nocsize) (rl : rule_name_t nocsize) : uaction (reg_t regno) (ext_fn_t interfacesize) := 
+(* to_action 0 H _ := { }; *)
+  to_action 1 (le_S n H1) _ with H1 := {} ; 
+  to_action nocsize H _  := to_action' nocsize _ _;
+
+
+  to_action _ H r with r := 
+to_action' (Nat.sub nocsize 1) H rl.
+
+
+Definition to_action rl :=
+match rl with
+| router_ idx => let idx_nat := index_to_nat idx in
+  if Nat.eqb idx_nat 0 then (routestartfn 0 (reg 0)) 
+  else if Nat.eqb idx_nat regno then (routeendfn regno (reg (Nat.sub regno 1))) 
+  else (routecenterfn idx_nat (reg (Nat.sub idx_nat 1)) (reg idx_nat))  
+end.
+ *)
+
+ 
+(* Fixpoint nat_to_fin {n : nat} (m : nat) : option (Fin.t n) :=
+  match n return option (Fin.t n) with
+  | 0 => None (* No valid index if the bound is 0 *)
+  | S n' => match m with
+            | 0 => Some Fin.F1 (* The 0th index corresponds to Fin.F1 *)
+            | S m' => match nat_to_fin m' with
+                      | Some fin' => Some (Fin.FS fin') (* Successor index *)
+                      | None => None
+                      end
+            end
+  end.
+
+Compute @nat_to_fin 4 2.
+
+Inductive reg_t (num : nat) : Type :=
+  | reg_ : Fin.t num -> reg_t num.
+
+Inductive rule_name_t (num : nat) : Type :=
+  | rule_ : Fin.t num -> rule_name_t num.
+
+Inductive ext_fn_t (num : nat) : Type :=
+  | ext_ : Fin.t num -> ext_fn_t num.
+
+
+(*How is num correctly determined*)
+Definition reg_fn (num : nat) (n : nat) : option (reg_t num) :=  
+    match Fin.of_nat n num with
+    | inleft fin_idx => Some (reg_ num fin_idx)  (* Valid index, return register *)
+    | inright _ => None  (* Index out of bounds, return None *)
+    end.
+
+Definition rule_fn (num : nat) (n : nat) : option (rule_name_t num) :=
+    match Fin.of_nat n num with
+    | inleft fin_idx => Some (rule_ num fin_idx)  (* Valid index, return register *)
+    | inright _ => None  (* Index out of bounds, return None *)
+    end.
+
+Definition e_fn (num : nat) (n : nat) : option (ext_fn_t num) :=
+    match Fin.of_nat n num with
+    | inleft fin_idx => Some (ext_ num fin_idx)  (* Valid index, return register *)
+    | inright _ => None  (* Index out of bounds, return None *)
+    end.
+
+Search Fin.t. 
+Compute rule_ 2 (Fin.FS Fin.F1).
+Check rule_fn nocsize 0.
+(* Axiom rego_ge_1 : regno >= 1. (*
+  unfold regno.
+  induction nocsize eqn:H.
+  - set (H1 := nocprop).
+    rewrite H in H1.
+    unfold ">"%nat in H1.
+    apply Nat.nlt_succ_diag_l in H1.
+    contradiction.
+  - apply IHn. *)
+Definition reg_of_nat (n:nat) :reg_t.
+  set (a := index_of_nat regno n).
+  destruct a eqn:H.
+  - exact (reg_ i).
+  - unfold a in H.
+    destruct regno eqn:H1.
+    + admit.
+    + simpl in H.
+    unfold index_of_nat in H.
+    Admitted.
+
+Print index_of_nat.
+Definition reg_of_nat n :=
+  reg_ (match index_of_nat regno n with
+        | Some n => n
+        | None => thisone
+        end). *)
+
+ (* Definition router n :=
+  router_ (match index_of_nat nocsize n with
+        | Some n => n
+        | None => thisone
+        end).   *)
+ 
+(* Compute index 3.
+Compute index_of_nat nocsize 1.
+
+
+Fixpoint list_seq_index_anotherone {N : nat} (l : list (index N)) : list (index (S N)) :=
+  match l with
+  | nil => nil
+  | cons el l' => cons (anotherone el) (list_seq_index_anotherone l')
+  end.
+
+(* Constucting an ascending list of all possible indecies N *)
+Fixpoint list_seq_index (N : nat) : list (index N) :=
+  match N with
+  | O => nil
+  | S N' => cons (thisone) (list_seq_index_anotherone (list_seq_index N'))
+  end. 
+  
+Fixpoint get_nth_item_fin {A : Type} (l : list A) (n : Fin.t regno) : A :=
+  match l with
+  | [] => match n with end (* This case is impossible due to the dependent type *)
+  | x :: xs =>
+    match n with
+    | Fin.F1 => x
+    | Fin.FS n' => get_nth_item_fin xs n'
+    end
+  end. *)
+
+Module MyRegs <: Registers.
+Definition reg_t:=reg_t regno.
+Definition ext_fn_t:= ext_fn_t regno.
+End MyRegs.
+
+Module Routerfns:= Router(MyRegs)(MyTypes).        
+Import Routerfns.
+
+Check rule_fn.
+
+Definition to_action (rl: rule_name_t nocsize) := 
+match rl with
+| (rule_fn nocsize 0) => routestartfn 0 reg_fn regno 0 reg_fn regno 1 extfn interfacesize 0 extfn interfacesize 1
+| rule_ => routecenterfn 1 r1 r2 r5 extfn_3 extfn_4
+| rule_ => routecenterfn 2 r2 r3 r6 extfn_5 extfn_6
+| rule_ => routeendfn 3 r3 r7 extfn_7 extfn_8
+end.
+
+
+Equations to_action
+ (rl : rule_name_t nocsize) : uaction (reg_t regno) (ext_fn_t interfacesize) := 
+to_action (rule_ nocsize) :=
+  let idx_nat := index_to_nat idx in
+  if Nat.eqb idx_nat 0 then
+    routestartfn 0 (reg_  indices 1)
+  else if Nat.eqb idx_nat regno then
+    let idx' := index_of_nat (Nat.sub idx_nat - 1) in
+    routeendfn regno (reg_ idx')
+  else
+    let idx' := index_of_nat (Nat.sub idx_nat - 1) in
+    routecenterfn idx_nat (reg_ idx') (reg_ idx).
+
+ *)
+
+ Definition t0_3: Fin.t 3:= @F1 2.
+ Definition t1_3: Fin.t 3:= @FS 2 (@F1 1).
+ Definition t2_3: Fin.t 3:= @FS 2 (@FS 1 (@F1 0)).
+
+ From Equations Require Import Equations.
+
+    
+ Module Type Number.
+   Parameter x: nat.
+   Axiom xprop: 1<x.
+ End Number.
+ 
+ Module Setup(ND:Number).
+   Import ND. 
+   Set Equations Debug.
+ 
+   Notation "!" := (False_rect _ _).
+ 
+   Equations? to_action (nocsize:nat) (H: 2<=nocsize) : nat :=
+      
+     to_action 1 (le_S nocsize H1) with H1 := {} ; 
+     to_action (S nocsize') H  := _.
+ 
+  Equations foo (x : nat) (H: 2<=x) (y : nat) : nat :=
+ 
+     foo 1 (le_S x H1) _ with H1 := {} ; 
+     foo x' H y' := x' + y'.
+ 
+  Equations foo (y : nat) : nat :=
+     foo y with xprop :=
+     foo y (le_S ?(0) H) := { ! };
+     foo y (le_S ?(1) (le_S ?(0) H)) := { ! }; 
+     foo y _ := x + y.
+ 
+ End Setup.
